theories/Base.v
@@ -47,13 +47,14 @@ From Katamaran Require Import
      Syntax.Terms
      Symbolic.Instantiation
      Symbolic.OccursCheck
+     Symbolic.GenOccursCheck
      Symbolic.PartialEvaluation.
 
 Module Type BaseMixin (Import TY : Types).
   Include
     ExpressionsOn TY <+
     TermsOn TY <+ PatternsOn TY <+
-    OccursCheckOn TY <+ InstantiationOn TY <+
+    OccursCheckOn TY <+ GenOccursCheckOn TY <+ InstantiationOn TY <+
     MessagesOn TY <+ PartialEvaluationOn TY.
 
   Notation Ty := (@ty.Ty typedeclkit).
